Reorganize (split into files).

theory/cwp/order.v
@@ -1,8 +1,30 @@
 Require Import Coq.Program.Basics.
+Require Import List.
 Require Import Coq.Relations.Relation_Definitions.
 Require Import Coq.Classes.RelationClasses.
 Require Import Coq.QArith.QArith.
+Require Import Coq.QArith.Qabs.
+Require Import Coq.micromega.Lqa.
+Require Import Coq.micromega.Lia.
 Local Open Scope program_scope.
+
+Require Import Q.
+
+
+(* Types with decidable equality *)
+Class EqType (A : Type) : Type :=
+  { eqb : A -> A -> bool
+  ; eqb_spec : forall x y, reflect (x = y) (eqb x y)
+  }.
+
+Instance EqType_bool : EqType bool :=
+  {| eqb := Bool.eqb
+   ; eqb_spec := Bool.eqb_spec |}.
+
+Instance EqType_nat : EqType nat :=
+  {| eqb := Nat.eqb
+   ; eqb_spec := Nat.eqb_spec |}.
+
 
 (* Ordered types *)
 Class OType (A : Type) : Type :=
@@ -22,13 +44,22 @@ Class PType (A : Type) `{o : OType A} : Type :=
   { bot : A
   ; bot_le : forall x, leq bot x }.
 
-
 Program Instance OType_arrow A B {oB : OType B} : OType (A -> B) :=
   {| leq := fun f g => forall x, leq (f x) (g x) |}.
 Next Obligation.
   constructor. firstorder.
   intros ?; etransitivity; eauto.
-Defined.
+Qed.
+
+Program Instance OType_nat : OType nat := {| leq := Nat.le |}.
+
+Program Instance OType_list A : OType (list A) :=
+  {| leq := fun l1 l2 => forall x, In x l1 -> In x l2 |}.
+Next Obligation. split; auto. Qed.
+
+Program Instance OType_Q : OType Q :=
+  { leq := Qle }.
+Next Obligation. Admitted.
 
 Program Instance PType_arrow A B `{p : PType B} : PType (A -> B) :=
   {| bot := const bot |}.
@@ -40,6 +71,16 @@ Definition equ {A : Type} `{OType A} (x y : A) :=
 (** f is an ω-chain *)
 Definition chain {A : Type} `{o : OType A} (f : nat -> A) : Prop :=
   forall i, leq (f i) (f (S i)).
+
+(** Apply all functions in a chain to the same argument x. *)
+Definition app_chain {A : Type} (ch : nat -> A -> Q) (x : A) : nat -> Q :=
+  flip ch x.
+
+Definition cons_chain {A : Type} (x : A) (ch : nat -> A) : nat -> A :=
+  fun i => match i with
+        | O => x
+        | S i' => ch i'
+        end.
 
 Definition lower_bound {A B : Type} `{OType B} (x : B) (f : A -> B) :=
   forall y, leq x (f y).
@@ -136,7 +177,6 @@ Lemma const_supremum' {A : Type} `{o : OType A} (f : nat -> A) (x : A) :
   supremum x f.
 Admitted.
 
-
 (* x is a fixed point of f *)
 Definition fixed_point {A : Type} (x : A) (f : A -> A) :=
   f x = x.
@@ -145,10 +185,6 @@ Definition fixed_point {A : Type} (x : A) (f : A -> A) :=
 Definition lfp {A : Type} `{OType A} (x : A) (f : A -> A) :=
   fixed_point x f /\ (forall y, fixed_point y f -> leq x y).
 
-Program Instance OType_Q : OType Q :=
-  { leq := Qle }.
-Next Obligation. Admitted.
-
 Lemma Qeq_equ (x y : Q) :
   x == y <-> equ x y.
 Proof.
@@ -156,9 +192,6 @@ Proof.
   - split; rewrite H; apply Qle_refl.
   - apply Qle_antisym; apply H.
 Qed.
-
-Notation "f '==f' g" := (forall x, f x == g x) (at level 80, no associativity) : order_scope.
-Local Open Scope order_scope.
 
 Lemma f_Qeq_equ {A : Type} (f g : A -> Q) :
   f ==f g <-> equ f g.
@@ -169,14 +202,116 @@ Proof.
   - intro x; apply Qeq_equ; split; apply H.
 Qed.
 
-Lemma f_Qeq_refl {A : Type} (f : A -> Q) :
-  f ==f f.
-Proof. intros; apply Qeq_refl. Qed.
 
-Lemma f_Qeq_trans {A : Type} (f g h : A -> Q) :
-  f ==f g -> g ==f h -> f ==f h.
-Proof. intros Hfg Hgh ?; rewrite Hfg; apply Hgh. Qed.
+Definition converges (g : nat -> Q) (lim : Q) :=
+  forall eps,
+    0 < eps ->
+    exists n0, forall n,
+        (n0 <= n)%nat -> Qabs (lim - g n) < eps.
 
-Lemma f_Qeq_symm {A : Type} (f g : A -> Q) :
-  f ==f g -> g ==f f.
-Proof. intros Hfg ?; rewrite Hfg; apply Qeq_refl. Qed.
+Lemma converges_increasing_ub (g : nat -> Q) (lim : Q) :
+  (forall i, g i <= g (S i)) ->
+  converges g lim ->
+  upper_bound lim g.
+Proof.
+  unfold converges.
+  intros Hle Hc n; simpl.
+  destruct (Qlt_le_dec lim (g n)); auto.
+  set (eps := g n - lim).
+  assert (0 < eps).
+  { unfold eps; lra. }
+  specialize (Hc eps H); destruct Hc as [n0 Hc].
+  specialize (Hc (max n n0) (Nat.le_max_r _ _)).
+  rewrite Qabs_Qminus in Hc.
+  assert (H0: forall m, (n <= m)%nat -> g n <= g m).
+  { intros m Hle'; induction m.
+    - inversion Hle'; lra.
+    - destruct (Nat.eqb_spec n (S m)); subst.
+      + lra.
+      + assert (n <= m)%nat. lia.
+        apply IHm in H0; eapply Qle_trans; eauto. }
+  assert (H1: g n <= g (max n n0)).
+  { apply H0. apply Nat.le_max_l. }
+  rewrite Qabs_Qminus_Qle in Hc.
+  - unfold eps in Hc; lra.
+  - lra.
+Qed.
+
+Lemma converges_increasing_le_ub (g : nat -> Q) (lim : Q) :
+  converges g lim ->
+  forall ub, upper_bound ub g -> lim <= ub.
+Proof.
+  unfold upper_bound; simpl; unfold converges.
+  intros Hc ub Hub; destruct (Qlt_le_dec ub lim); auto.
+  set (eps := lim - ub).
+  assert (Heps: 0 < eps).
+  { unfold eps; lra. }
+  specialize (Hc eps Heps); destruct Hc as [n0 Hc].
+  specialize (Hc n0 (le_refl _)); specialize (Hub n0).
+  unfold eps in Hc; rewrite Qabs_Qminus_Qle in Hc; lra.
+Qed.
+
+(* If g is monotonically increasing and converges to lim, then lim is
+   the supremum of g. *)
+Lemma converges_from_below_supremum (g : nat -> Q) (lim : Q) :
+  (forall i, g i <= g (S i)) ->
+  converges g lim ->
+  supremum lim g.
+Proof.
+  unfold converges.
+  intros Hc. split.
+  - apply converges_increasing_ub; auto.
+  - apply converges_increasing_le_ub; auto.
+Qed.
+
+Lemma Proper_converges : Proper (f_Qeq ==> Qeq ==> iff) converges.
+Proof.
+  intros f g Heq1 x y Heq2.
+  unfold converges.
+  split; intros Hc eps Heps.
+  - destruct (Hc eps Heps) as [n0 Hc'].
+    exists n0; intros n Hle; apply Hc' in Hle; rewrite <- Heq2.
+    specialize (Heq1 n); rewrite <- Heq1; auto.
+  - destruct (Hc eps Heps) as [n0 Hc'].
+    exists n0; intros n Hle; apply Hc' in Hle; rewrite Heq2.
+    specialize (Heq1 n); rewrite Heq1; auto.
+Qed.
+
+(** Not an actual Proper instance because it can be defined more
+    generally. Although I guess it doesn't matter. *)
+Lemma Proper_supremum_Q : Proper (Qeq ==> @f_Qeq nat ==> iff) supremum.
+Proof.
+  unfold f_Qeq. intros x y Heq1 f g Heq2. unfold supremum, upper_bound, leq; simpl.
+  split; intros [Hub Hlub].
+  - split.
+    + intro z; rewrite <- Heq1, <- Heq2; auto.
+    + intros z Hle; rewrite <- Heq1; apply Hlub; intro w; rewrite Heq2; auto.
+  - split.
+    + intro z; rewrite Heq1, Heq2; auto.
+    + intros z Hle; rewrite Heq1; apply Hlub; intro w; rewrite <- Heq2; auto.
+Qed.
+
+(** Given a function f and a chain of functions g, f is the supremum
+    of g if forall x, f x is the supremum of g specialized to x. *)
+Lemma supremum_pointwise {A : Type} (ch : nat -> A -> Q) (f : A -> Q) :
+  (forall x, supremum (f x) (app_chain ch x)) ->
+  supremum f ch.
+Proof.
+  intro Hsup; split.
+  - intros ? ?; apply Hsup.
+  - intros ? Hub ?; apply Hsup; intros ?; apply Hub.
+Qed.
+
+Lemma cons_chain_supremum {A : Type} `{OType A} (x : A) (ch : nat -> A) (sup : A) :
+  (forall i, leq x (ch i)) ->
+  supremum sup ch ->
+  supremum sup (cons_chain x ch).
+Proof.
+  unfold supremum, upper_bound.
+  intros Hleq [Hub Hlub]; split.
+  - intro y. destruct y; simpl; auto.
+    destruct H as [le [Hrefl Htrans]].
+    eapply Htrans. apply (Hleq O). apply Hub.
+  - intros ub Hub'. apply Hlub; intro z.
+    specialize (Hub' (S z)); apply Hub'.
+Qed.
