theory/cwp/cwp_infer.v
@@ -1,0 +1,208 @@
+Set Implicit Arguments.
+
+Require Import Coq.Program.Basics.
+Require Import Coq.QArith.QArith.
+Require Import Coq.micromega.Lia.
+Require Import ExtLib.Data.Monads.StateMonad.
+Local Open Scope program_scope.
+
+Require Import compile.
+Require Import cpGCL.
+Require Import cwp.
+Require Import infer.
+Require Import order.
+Require Import tree.
+
+Theorem wp_infer (c : cpGCL) (f : St -> Q) (n : nat) :
+  wf_cpGCL c ->
+  expectation f ->
+  wp c f (infer_f f ∘ evalCompile c n).
+Proof.
+  revert f n. induction c; intros f m Hwf Hexp; try solve [constructor; intros ?; reflexivity].
+  (* sequence *)
+  - unfold compose. unfold evalCompile, evalState in *. simpl.
+    destruct (runState (compile c1) m) eqn:Hc1.
+    destruct (runState (compile c2) n) eqn:Hc2.
+    inversion Hwf; subst.
+    econstructor. apply IHc2 with (n:=n); auto.
+    apply IHc1 with (n:=m); auto. intro x.
+    apply infer_f_expectation_0_le; auto. apply compile_wf; auto.
+    intro x. unfold compose. simpl.
+    rewrite Hc1. rewrite Hc2.
+    unfold kcomp. simpl. rewrite <- infer_f_bind. reflexivity.
+    intros n1 x0 Hbound. eapply compile_bound_in_not_in.
+    apply Hc1. apply Hc2. omega. apply Hbound.
+  (* ite *)
+  - unfold compose; simpl.
+    set (fi := infer_f f).
+    inversion Hwf; subst.
+    unfold evalCompile, evalState in *. simpl.
+    destruct (runState (compile c1) m) eqn:Hc1.
+    destruct (runState (compile c2) n) eqn:Hc2. simpl.
+    econstructor. apply IHc1 with (n:=m); auto.
+    apply IHc2 with (n:=n); auto.
+    intro x. destruct (e x).
+    rewrite Hc1; reflexivity.
+    rewrite Hc2; reflexivity.
+  (* choice *)
+  - unfold compose, evalCompile, evalState in *; simpl.
+    inversion Hwf; subst.
+    specialize (IHc1 f m H3 Hexp).
+    destruct (runState (compile c1) m) eqn:Hc1.
+    specialize (IHc2 f n H4 Hexp).
+    destruct (runState (compile c2) n) eqn:Hc2. simpl in *.
+    econstructor.
+    apply IHc1.
+    apply IHc2.
+    reflexivity.
+  (* while *)
+  -
+    (* Need to provide a chain of approximations that satisfies the
+       conditions of the while wp constructor, and such that infer
+       after compile yields of the supremum of that chain (probably
+       via an argument based on convergence of geometric series). *)
+    simpl. unfold compose. simpl.
+    unfold evalCompile, evalState.
+    simpl. destruct (runState (compile c) (S m)) eqn:Hc. simpl.
+    rename t into k.
+    set (k' := fun st => tree_bind (k st) (fun st' => if e st' then Fail _ (S m) else Leaf st')).
+    set (ch := fun i => fun st => infer_f f (tree_chain (k' st ) (S m) i)).
+    set (ch' := cons_chain (const 0) ch).
+    apply wp_while with ch'.
+    + reflexivity.
+    + admit. (* TODO: prove chain is ω-invariant *)
+    + unfold ch'. apply cons_chain_supremum.
+      * unfold ch.
+        intros i st; unfold const; simpl.
+        apply infer_f_expectation_0_le; auto.
+        apply tree_chain_wf. unfold k'.
+        apply compile_wf with (n:=m) (st:=st) in Hwf.
+        unfold evalCompile, evalState in Hwf. simpl in Hwf.
+        unfold k'. (* unfold k. *)
+        apply wf_tree_bind; auto.
+        ++ intros. apply bound_in_not_bound_in; intro HC.
+           destruct (e x); inversion HC.
+        ++ rewrite Hc in Hwf. simpl in Hwf.
+           inversion Hwf; subst; eapply wf_tree_bind'; eauto.
+        ++ intros; destruct (e x); constructor.
+      * unfold ch.
+        unfold k'.
+        apply infer_f_supremum_expectation; auto.
+        { intro st.
+          apply wf_tree'_bind.
+          - intros ? ? ? ? HC; destruct (e x); inversion HC.
+          - intros n0 m0 x Hbound Hfree.
+            destruct (e x); inversion Hfree; subst.
+            eapply compile_bound_labels in Hc; eauto; lia.
+          - inversion Hwf; subst.
+            apply compile_wf_tree' with (c:=c) (m:=S m) (n:=n); auto.
+          - intros; destruct (e x); constructor. }
+        { intros st l Hbound.
+          apply bound_in_bind in Hbound. destruct Hbound as [Hbound|[x HC]].
+          - eapply compile_bound_labels in Hc; eauto; lia.
+          - destruct (e x); inversion HC. }
+        { intros st n0 m0 Hbound Hfree.
+          apply bound_in_bind in Hbound. destruct Hbound as [Hbound | [x HC]].
+          - apply free_in_bind in Hfree. destruct Hfree as [Hfree | [x Hfree]].
+            * pose proof Hc as Hc'.
+              eapply compile_bound_labels in Hc; eauto.
+              eapply compile_free_in_0 in Hc'; eauto; subst.
+              lia.
+            * destruct (e x); inversion Hfree; subst.
+              eapply compile_bound_labels in Hc; eauto; lia.
+          - destruct (e x); inversion HC. }
+  (* observe *)
+  - unfold compose, evalCompile, evalState; simpl.
+    constructor. intro x. destruct (e x); reflexivity.
+Admitted.
+
+Theorem wlp_infer (c : cpGCL) (f : St -> Q) (n : nat) :
+  wf_cpGCL c ->
+  expectation f ->
+  wlp c f (infer_f_lib f ∘ evalCompile c n).
+Admitted.
+
+Theorem cwp_infer (c : cpGCL) (f : St -> Q) :
+  wf_cpGCL c ->
+  expectation f ->
+  cwp c f (infer f ∘ evalCompile' c).
+Proof.
+  intros Hwf Hexp.
+  eexists; eexists; split.
+  - split.
+    + apply wp_infer with (n:=O); auto.
+    + apply wlp_infer with (n:=O); auto.
+      compute; congruence.
+  - reflexivity.
+Qed.
+
+Lemma wp_iid_infer_f c f n :
+  wf_cpGCL c ->
+  wp_iid c f ==f infer_f f ∘ evalCompile c n.
+Proof.
+  revert n f.
+  induction c; intros m f Hwf st;
+    unfold evalCompile, evalState, compose; simpl; inversion Hwf; subst.
+  - reflexivity.
+  - rewrite Qdiv_0_num; reflexivity.
+  - reflexivity.
+  - unfold compose.
+    unfold compose, f_Qeq, evalCompile, evalState in *.
+    destruct (runState (compile c1) m) eqn:Hc1.
+    destruct (runState (compile c2) n) eqn:Hc2.
+    specialize (IHc1 m (wp_iid c2 f) H1 st).
+    rewrite IHc1. simpl.
+    rewrite Hc1. simpl.
+    unfold kcomp. simpl.
+    rewrite <- infer_f_bind. unfold compose. simpl.
+    + apply infer_f_proper; intro x.
+      specialize (IHc2 n f H2 x).
+      rewrite IHc2, Hc2; reflexivity.
+    + intros l x Hbound. apply not_in_not_bound_and_not_free. split.
+      * apply free_in_not_free_in; intro HC.
+        eapply compile_free_in_0 in Hc2; eauto. subst.
+        eapply compile_bound_labels in Hc1; eauto; lia.
+      * apply bound_in_not_bound_in; intro HC.
+        eapply compile_bound_labels in Hc2; eauto.
+        eapply compile_bound_labels in Hc1; eauto.
+        lia.
+  - unfold compose, evalCompile, evalState, f_Qeq in *.
+    destruct (runState (compile c1) m) eqn:Hc1.
+    destruct (runState (compile c2) n) eqn:Hc2.
+    simpl; destruct (e st).
+    + rewrite IHc1, Hc1; auto; reflexivity.
+    + rewrite IHc2, Hc2; auto; reflexivity.
+  - unfold compose, evalCompile, evalState, f_Qeq in *.
+    destruct (runState (compile c1) m) eqn:Hc1.
+    destruct (runState (compile c2) n) eqn:Hc2.
+    rewrite IHc1, Hc1, IHc2, Hc2; auto; reflexivity.
+  - destruct (runState (compile c) (S m)) eqn:Hc.
+    pose proof IHc as IHc'.
+    specialize (IHc (S m) f H0 st).
+    unfold compose, evalCompile, evalState, f_Qeq in *.
+    rewrite Hc in IHc. simpl in *.
+    set (g := fun st' => if e st' then 0 else f st').
+    set (h := fun st' => if e st' then 1 else 0).
+    set (k := fun st' => if e st' then Fail St (S m) else Leaf st').
+    cut (wp_iid c g st == infer_f f (tree_bind (t st) k)).
+    cut (wp_iid c h st == infer_fail (S m) (tree_bind (t st) k)).
+    { intros H1 H2; rewrite H1, H2; reflexivity. }
+    + unfold h. unfold k.
+      rewrite infer_fail_tree_bind_infer_f.
+      specialize (IHc' (S m) (fun st => if e st then 1 else 0) H0 st).
+      rewrite Hc in IHc'. simpl in IHc'.
+      apply IHc'.
+      apply label_in_not_in; intro HC. apply label_in_bound_or_free in HC.
+      destruct HC as [HC|HC].
+      * eapply compile_bound_labels in Hc; eauto; lia.
+      * eapply compile_free_in_0 in Hc; eauto; lia.
+      * eapply compile_wf_tree'; eauto.
+    + specialize (IHc' (S m) g H0 st).
+      rewrite IHc'. rewrite Hc. simpl.
+      unfold g. unfold k.
+      rewrite infer_f_tree_bind.
+      * reflexivity.
+      * apply bound_in_not_bound_in; intro HC.
+        eapply compile_bound_labels in Hc; eauto; lia.
+  - destruct (e st); reflexivity.
+Qed.
