theory/cwp/geometric.v
@@ -1,0 +1,146 @@
+Set Implicit Arguments.
+Require Import List.
+Require Import Coq.QArith.QArith.
+Require Import Coq.micromega.Lqa.
+Require Import Coq.micromega.Lia.
+
+Require Import order.
+Require Import Q.
+
+Fixpoint geometric_series (a r : Q) (n : nat) :=
+  match n with
+  | O => a
+  | S n' => geometric_series a r n' + a * Qpow r n
+  end.
+
+Definition geometric_series' (a r : Q) (n : nat) : Q :=
+  sum_Q_list (map (fun n => a * Qpow r n) (seq O (S n))).
+
+Lemma geometric_series_geometric_series' (a r : Q) (n : nat) :
+  geometric_series a r n == geometric_series' a r n.
+Proof.
+  unfold geometric_series'.
+  induction n.
+  - simpl; field.
+  - simpl in *.
+    rewrite IHn. ring_simplify.
+    set (f := fun n => a * Qpow r n).
+    assert (a == f O).
+    { unfold f. simpl. field. }
+    rewrite H.
+    rewrite <- Qplus_assoc.
+    rewrite sum_Q_list_l.
+    rewrite Qplus_comm.
+    simpl.
+    assert (H0: f O * r * Qpow r n == f (1 + n)%nat).
+    { unfold f. simpl. field. }
+    rewrite H0.
+    rewrite <- Qplus_assoc.
+    rewrite sum_Q_list_r.
+    unfold f. simpl. field.
+Qed.
+
+(* In general we require (|r| < 1) to ensure convergence, but here we
+   assume the stronger condition (0 <= r < 1) for simplicity and
+   because r will always be nonnegative for our purposes. *)
+Axiom geometric_series_converges :
+  forall a r,
+    0 <= r -> r < 1 ->
+    converges (geometric_series a r) (a / (1 - r)).
+
+(* Definition converges_from_below (g : nat -> Q) (lim : Q) := *)
+(*   forall eps, 0 < eps -> *)
+(*          exists n0, forall n, *)
+(*              (n0 <= n)%nat -> lim - g n < eps. *)
+
+(* Axiom geometric_series_converges : *)
+(*   forall a r, converges (geometric_series a r) (a / (1 - r)). *)
+
+(* Axiom geometric_series_converges : *)
+(*   forall a r eps, *)
+(*     0 <= a <= 1 -> 0 <= r -> r < 1 -> 0 < eps -> *)
+(*     exists n0, forall n, *)
+(*         (n0 <= n)%nat -> (a / (1 - r)) - geometric_series a r n < eps. *)
+
+(* Definition prefix_series {A : Type} (n : nat) (f : nat -> A) (i : nat) := *)
+(*   f (i-n)%nat. *)
+
+(* Definition postfix_series {A : Type} (n : nat) (f : nat -> A) (i : nat) := *)
+(*   f (i-n)%nat. *)
+
+Lemma geometric_series_succ (a r : Q) (n : nat) :
+  a + r * geometric_series a r n == geometric_series a r (S n).
+Proof.
+  rewrite 2!geometric_series_geometric_series'.
+  unfold geometric_series'. simpl.
+  set (f := fun i => a * Qpow r i).
+  assert (H0: a * 1 == f O).
+  { reflexivity. }
+  rewrite H0.
+  rewrite sum_Q_list_l.
+  assert (H1: a * (r * 1) == f (S O)).
+  { reflexivity. }
+  rewrite H1.
+  rewrite sum_Q_list_l. rewrite sum_Q_list_l.
+  rewrite sum_Q_list_distr. unfold f.
+  rewrite sum_Q_list_Qpow; simpl; field.
+Qed.
+
+Lemma geometric_series_supremum (a r : Q) :
+  0 <= a ->
+  0 <= r -> r < 1 ->
+  supremum (a / (1 - r)) (geometric_series a r).
+Proof.
+  intros; apply converges_from_below_supremum.
+  - intro i. simpl.
+    assert (0 <= Qpow r i).
+    { apply Qpow_nonnegative; auto. }
+    assert (0 <= r * Qpow r i). nra. nra.
+  - apply geometric_series_converges; auto.
+Qed.
+
+Lemma geometric_series_monotone (a r : Q) :
+  (0 <= a) -> (0 <= r) ->
+  monotone (geometric_series a r).
+Proof.
+  intros Hle_a Hle_r n m Hleq. simpl in *.
+  induction m. simpl.
+  - inversion Hleq; subst; simpl; lra.
+  - unfold Nat.le in *.
+    destruct (Nat.eqb_spec n (S m)); subst. lra.
+    assert (Hle: (n <= m)%nat). lia.
+    apply IHm in Hle. simpl.
+    generalize (@Qpow_nonnegative r m Hle_r).
+    intro Hle_pow.
+    assert (0 <= r * Qpow r m); nra.
+Qed.
+
+Lemma geometric_supremum (ch : nat -> Q) (a r : Q) :
+  0 <= a ->
+  0 <= r -> r < 1 ->
+  ch ==f geometric_series a r ->
+  supremum (a / (1 - r)) ch.
+Proof.
+  intros Hle_a Hle_r0 Hle_r1 Heq.
+  apply converges_from_below_supremum.
+  - intro i. unfold f_Qeq in Heq. rewrite 2!Heq.
+    apply geometric_series_monotone; auto; simpl; unfold Nat.le; lia.
+  - eapply Proper_converges; eauto. reflexivity.
+    apply geometric_series_converges; auto.
+Qed.
+
+Instance Proper_geometric_series
+  : Proper (Qeq ==> Qeq ==> eq ==> Qeq) geometric_series.
+Proof.
+  intros a b Heq1 c d Heq2 n m Heq3.
+  subst. induction m; simpl; auto.
+  rewrite IHm, Heq1, Heq2; reflexivity.
+Qed.
+
+Lemma geometric_series_const (a : Q) (n : nat) :
+  geometric_series a 0 n == a.
+Proof.
+  induction n; simpl.
+  - reflexivity.
+  - rewrite IHn; lra.
+Qed.
