theory/cwp/misc.v
@@ -1,0 +1,34 @@
+Set Implicit Arguments.
+
+Require Import PeanoNat.
+Require Import List.
+Require Import Coq.micromega.Lia.
+
+Require Import order.
+
+Definition list_max (l : list nat) : nat := fold_right max O l.
+
+Lemma list_max_spec (l : list nat) (x : nat) :
+  In x l ->
+  (x <= list_max l)%nat.
+Proof.
+  induction l; intro Hin.
+  - inversion Hin.
+  - destruct Hin as [H|H]; subst; simpl.
+    + apply Nat.le_max_l.
+    + etransitivity. apply IHl; auto.
+      apply Nat.le_max_r.
+Qed.
+
+Lemma list_max_monotone : monotone (list_max).
+Proof.
+  intros l1 l2; unfold leq; simpl; intro Hleq; unfold Nat.le.
+  induction l1; simpl.
+  - lia.
+  - destruct (Nat.leb_spec a (list_max l1)).
+    + rewrite max_r; auto; apply IHl1.
+      intros x Hin. apply Hleq. right; auto.
+    + rewrite max_l.
+      * apply list_max_spec; apply Hleq; left; auto.
+      * lia.
+Qed.
