theory/cwp/tests.v
@@ -1,0 +1,126 @@
+Set Implicit Arguments.
+
+Require Import Coq.Program.Basics.
+Require Import Coq.QArith.QArith.
+
+Require Import compile.
+Require Import cpGCL.
+Require Import cwp.
+Require Import infer.
+Require Import tree.
+
+(** Testing compilation and inference on example programs *)
+
+Definition sample (x : nat) (p : Q) : cpGCL :=
+  CChoice p (CAssign x (const true)) (CAssign x (const false)).
+
+Definition goldfish_piranha : cpGCL :=
+  sample 0%nat (1#2) ;;
+  CAssign 1%nat (const true) ;;
+  CChoice (1#2) (CAssign 2%nat (fun st => st 0%nat))
+                (CAssign 2%nat (fun st => st 1%nat)) ;;
+  CObserve (fun st => eqb (st 2%nat) true).
+
+Definition goldfish_piranha_tree : tree St :=
+  evalCompile' goldfish_piranha empty.
+
+Definition ex1_f := fun st => if st O : bool then 1 else 0.
+Example ex1 : infer ex1_f goldfish_piranha_tree == 2#3.
+Proof. reflexivity. Qed.
+Example ex2 : infer ex1_f goldfish_piranha_tree ==
+              cwp_iid goldfish_piranha ex1_f empty.
+Proof. reflexivity. Qed.
+
+Definition test_abort : cpGCL :=
+  CChoice (1#3) (CAssign 0%nat (const true)) CAbort.
+
+Definition test_abort_tree : tree St := evalCompile' test_abort empty.
+
+(* Eval compute in (evalCompile' test_abort empty). *)
+
+Definition ex3_f := fun st => if st O : bool then 1 else 0.
+Example ex3 : infer ex3_f test_abort_tree == 1#3.
+Proof. reflexivity. Qed.
+Example ex4 : infer ex3_f test_abort_tree == cwp_iid test_abort ex3_f empty.
+Proof. reflexivity. Qed.
+
+Definition ex5_f := fun st => if st O : bool then 1 else 0.
+Example ex5 : infer ex5_f test_abort_tree == 1#3.
+Proof. reflexivity. Qed.
+Example ex6 : infer ex5_f test_abort_tree == cwp_iid test_abort ex5_f empty.
+Proof. reflexivity. Qed.
+
+Definition ex7_f := fun st => if negb (st O) then 1 else 0.
+Example ex7 : infer ex7_f test_abort_tree == 0.
+Proof. reflexivity. Qed.
+Example ex8 : infer ex7_f test_abort_tree == cwp_iid test_abort ex7_f empty.
+Proof. reflexivity. Qed.
+
+Example ex9 : infer (const 1) test_abort_tree == 1#3.
+Proof. reflexivity. Qed.
+Example ex10 : infer (const 1) test_abort_tree ==
+               cwp_iid test_abort (const 1) empty.
+Proof. reflexivity. Qed.
+
+(** infer_f (const 1) yields the probability of terminating. *)
+Example ex11 : infer_f (const 1) test_abort_tree == 1#3.
+Proof. reflexivity. Qed.
+(** infer_f_lib (const 1) always yields 1. *)
+Example ex12 : infer_f_lib (const 1) test_abort_tree == 1.
+Proof. reflexivity. Qed.
+
+Definition ex13_f := fun st => if st O : bool then 1 else 0.
+Example ex13 : infer ex13_f test_abort_tree == 1#3.
+Proof. reflexivity. Qed.
+Example ex14 : infer ex13_f test_abort_tree ==
+               cwp_iid test_abort ex13_f empty.
+Proof. reflexivity. Qed.
+
+Definition ex15_c := CChoice (1#2) CSkip CAbort.
+Example ex15 : infer (const 1) (evalCompile' ex15_c empty) == 1#2.
+Proof. reflexivity. Qed.
+Example ex16 : infer (const 1) (evalCompile' ex15_c empty) ==
+               cwp_iid ex15_c (const 1) empty.
+Proof. reflexivity. Qed.
+
+Definition fair_coin : cpGCL :=
+  CAssign 0 (const false) ;;
+  CAssign 1 (const false) ;;
+  CWhile (fun st => eqb (st 0%nat) (st 1%nat))
+         (sample 0%nat (1#3) ;; sample 1%nat (1#3)).
+
+Definition fair_coin_tree : tree St := evalCompile' fair_coin empty.
+
+Definition ex17_f := fun st => if st O : bool then 1 else 0.
+Example ex17 : infer ex17_f fair_coin_tree == 1#2.
+Proof. reflexivity. Qed.
+Example ex18 : infer ex17_f fair_coin_tree == cwp_iid fair_coin ex17_f empty.
+Proof. reflexivity. Qed.
+
+Definition two_thirds_loop (x : nat) (z : nat) : cpGCL :=
+  CAssign z (const true) ;;
+    CWhile (fun st => st z)
+           (CChoice (1#2)
+                    (CAssign x (const true) ;;
+                     CAssign z (const false))
+                    (CChoice (1#2)
+                             CSkip
+                             (CAssign x (const false) ;;
+                              CAssign z (const false)))).
+
+Definition fair_coin_loop : cpGCL :=
+  CAssign 0 (const false) ;;
+  CAssign 1 (const false) ;;
+  CWhile (fun st => eqb (st 0%nat) (st 1%nat))
+         (two_thirds_loop 0%nat 2%nat ;;
+          two_thirds_loop 1%nat 2%nat).
+
+Definition fair_coin_loop_tree : tree St := evalCompile' fair_coin_loop empty.
+
+Definition ex19_f := fun st => if st O : bool then 1 else 0.
+Example ex19 : infer ex19_f fair_coin_loop_tree == 1#2.
+Proof. reflexivity. Qed.
+Example ex20 : infer ex19_f fair_coin_loop_tree ==
+               cwp_iid fair_coin_loop ex19_f empty.
+Proof. reflexivity. Qed.
+
