theory/cwp/tree.v
@@ -1,0 +1,1419 @@
+Set Implicit Arguments.
+Require Import Coq.Program.Basics.
+Require Import List.
+Require Import Coq.QArith.QArith.
+Require Import Coq.micromega.Lqa.
+Require Import Coq.micromega.Lia.
+Require Import ExtLib.Structures.Monad.
+Import ListNotations.
+
+Require Import misc.
+Require Import order.
+
+(** Choice trees with fix (loop) nodes ("fix trees"?) *)
+Inductive tree (A : Type) : Type :=
+| Leaf : A -> tree A
+| Fail : nat -> tree A
+| Choice : Q -> tree A -> tree A -> tree A
+| Fix : nat -> tree A -> tree A.
+
+Fixpoint fmap {A B : Type} (f : A -> B) (t : tree A) : tree B :=
+  match t with
+  | Leaf x => Leaf (f x)
+  | Fail _ n => Fail _ n
+  | Choice p t1 t2 => Choice p (fmap f t1) (fmap f t2)
+  | Fix l t => Fix l (fmap f t)
+  end.
+
+Fixpoint join {A : Type} (t : tree (tree A)) : tree A :=
+  match t with
+  | Leaf t' => t'
+  | Fail _ n => Fail _ n
+  | Choice p t1 t2 => Choice p (join t1) (join t2)
+  | Fix l t => Fix l (join t)
+  end.
+
+Definition tree_bind {A B : Type} (t : tree A) (k : A -> tree B) : tree B :=
+  join (fmap k t).
+
+Instance Monad_tree : Monad tree := { ret := Leaf; bind := @tree_bind }.
+
+Definition kcomp {A B C : Type} (f : A -> tree B) (g : B -> tree C) : A -> tree C :=
+  fun x => bind (f x) g.
+
+(** Like bind but extending fail nodes instead of leaves. *)
+Fixpoint fbind {A : Type} (n : nat) (t1 t2 : tree A) : tree A :=
+  match t1 with
+  | Leaf x => Leaf x
+  | Fail _ m => if n =? m then t2 else Fail _ m
+  | Choice p t' t'' => Choice p (fbind n t' t2) (fbind n t'' t2)
+  | Fix l t => Fix l (if l =? n then t else fbind n t t2)
+  end.
+
+Fixpoint bound_labels {A : Type} (t : tree A) : list nat :=
+  match t with
+  | Choice _ t1 t2 => nodup Nat.eq_dec (bound_labels t1 ++ bound_labels t2)
+  | Fix l t => nodup Nat.eq_dec (l :: bound_labels t)
+  | _ => []
+  end.
+
+Fixpoint all_labels {A : Type} (t : tree A) : list nat :=
+  match t with
+  | Leaf _ => []
+  | Fail _ l => [l]
+  | Choice _ t1 t2 => nodup Nat.eq_dec (all_labels t1 ++ all_labels t2)
+  | Fix l t => nodup Nat.eq_dec (l :: all_labels t)
+  end.
+
+Fixpoint subst_l {A : Type} (x y : nat) (t : tree A) : tree A :=
+  match t with
+  | Leaf x => Leaf x
+  | Fail _ l => Fail _ (if l =? x then y else l)
+  | Choice p t1 t2 => Choice p (subst_l x y t1) (subst_l x y t2)
+  | Fix l t1 => Fix l (if l =? x then t1 else subst_l x y t1)
+  end.
+
+Fixpoint alpha_convert {A : Type} (f : nat -> nat) (t : tree A) : tree A :=
+  match t with
+  | Choice p t1 t2 => Choice p (alpha_convert f t1) (alpha_convert f t2)
+  | Fix l t => Fix (f l) (subst_l l (f l) (alpha_convert f t))
+  | _ => t
+  end.
+
+Fixpoint tree_chain {A : Type} (t : tree A) (l i : nat) : tree A :=
+  match i with
+  | O => t
+  (* | S i' => fbind l (tree_chain t l i') (freshen_labels i t) *)
+  | S i' =>
+    let ti' := tree_chain t l i' in
+    fbind l ti' (alpha_convert
+                   (fun x => (x + list_max (all_labels ti') + 1)%nat) t)
+  end.
+
+Inductive tree_eq {A : Type} : tree A -> tree A -> Prop :=
+| tree_eq_leaf : forall x, tree_eq (Leaf x) (Leaf x)
+| tree_eq_fail : forall l, tree_eq (Fail _ l) (Fail _ l)
+| tree_eq_choice : forall p q t1 t1' t2 t2',
+    p == q ->
+    tree_eq t1 t1' ->
+    tree_eq t2 t2' ->
+    tree_eq (Choice p t1 t2) (Choice q t1' t2')
+| tree_eq_fix : forall l t1 t2,
+    tree_eq t1 t2 ->
+    tree_eq (Fix l t1) (Fix l t2).
+
+Fixpoint tree_eqb {A : Type} `{EqType A} (t1 t2 : tree A) : bool :=
+  match (t1, t2) with
+  | (Leaf x, Leaf y) => eqb x y
+  | (Fail _ n, Fail _ m) => eqb n m
+  | (Choice p tl tr, Choice q tl' tr') =>
+    match Qeq_dec p q with
+    | left _ => tree_eqb tl tl' && tree_eqb tr tr'
+    | right _ => false
+    end
+  | (Fix n t1', Fix m t2') => eqb n m && tree_eqb t1' t2'
+  | _ => false
+  end.
+
+Lemma tree_eqb_spec {A : Type} `{EqType A} (t1 t2 : tree A)
+  : reflect (tree_eq t1 t2) (tree_eqb t1 t2).
+Proof.
+  revert t2. induction t1; intro t2.
+  - destruct t2; simpl; try solve [right; intro HC; inversion HC].
+    destruct (eqb_spec a a0); subst.
+    + left; constructor.
+    + right; intro HC; inversion HC; subst; congruence.
+  - destruct t2; simpl; try solve [right; intro HC; inversion HC].
+    destruct (Nat.eqb_spec n n0); subst.
+    + left; constructor.
+    + right; intro HC; inversion HC; subst; congruence.
+  - destruct t2; simpl; try constructor; try solve [intro HC; inversion HC].
+    destruct (Qeq_dec q q0).
+    + destruct (IHt1_1 t2_1); destruct (IHt1_2 t2_2); simpl;
+        try (left; constructor; auto); right; intro HC;
+          inversion HC; subst; congruence.
+    + right; intro HC; inversion HC; subst; congruence.
+  - destruct t2; simpl; try (right; intro HC; inversion HC).
+    destruct (Nat.eqb_spec n n0); subst; simpl.
+    + destruct (IHt1 t2); constructor.
+      * constructor; auto.
+      * intro HC; inversion HC; subst; congruence.
+    + right; intro HC; inversion HC; subst; congruence.
+Qed.
+
+Inductive tree_leq {A : Type} : tree A -> tree A -> Prop :=
+| tree_leq_leaf : forall x, tree_leq (Leaf x) (Leaf x)
+| tree_leq_fail : forall l t, tree_leq (Fail _ l) t
+| tree_leq_choice : forall p q t1 t1' t2 t2',
+    p == q ->
+    tree_leq t1 t1' ->
+    tree_leq t2 t2' ->
+    tree_leq (Choice p t1 t2) (Choice q t1' t2')
+| tree_leq_fix : forall l t1 t2,
+    tree_leq t1 t2 ->
+    tree_leq (Fix l t1) (Fix l t2).
+
+Fixpoint tree_leqb {A : Type} `{EqType A} (t1 t2 : tree A) : bool :=
+  match (t1, t2) with
+  | (Leaf x, Leaf y) => eqb x y
+  | (Fail _ n, _) => true
+  | (Choice p tl tr, Choice q tl' tr') =>
+    match Qeq_dec p q with
+    | left _ => tree_leqb tl tl' && tree_leqb tr tr'
+    | right _ => false
+    end
+  | (Fix n t1', Fix m t2') => eqb n m && tree_leqb t1' t2'
+  | _ => false
+  end.
+
+Lemma tree_leqb_spec {A : Type} `{EqType A} (t1 t2 : tree A)
+  : reflect (tree_leq t1 t2) (tree_leqb t1 t2).
+Proof.
+  revert t2. induction t1; intro t2.
+  - destruct t2; simpl; try solve [right; intro HC; inversion HC].
+    destruct (eqb_spec a a0); subst.
+    + left; constructor.
+    + right; intro HC; inversion HC; subst; congruence.
+  - destruct t2; simpl; left; constructor.
+  - destruct t2; simpl; try constructor; try solve [intro HC; inversion HC].
+    destruct (Qeq_dec q q0).
+    + destruct (IHt1_1 t2_1); destruct (IHt1_2 t2_2); simpl;
+        try (left; constructor; auto); right; intro HC;
+          inversion HC; subst; congruence.
+    + right; intro HC; inversion HC; subst; congruence.
+  - destruct t2; simpl; try (right; intro HC; inversion HC).
+    destruct (Nat.eqb_spec n n0); subst; simpl.
+    + destruct (IHt1 t2); constructor.
+      * constructor; auto.
+      * intro HC; inversion HC; subst; congruence.
+    + right; intro HC; inversion HC; subst; congruence.
+Qed.
+
+(** Not true unless we change tree_leq to be slightly less permissive
+    in the fail case. *)
+(* Lemma tree_eq_leq {A : Type} (t1 t2 : tree A) : *)
+(*   tree_eq t1 t2 <-> tree_leq t1 t2 /\ tree_leq t2 t1. *)
+(* Proof. *)
+(*   split. *)
+(*   - intro Heq. induction Heq; split; constructor; intuition. *)
+(*   - intros [Hleq0 Hleq1]. *)
+(*     + inversion Hleq0; subst; inversion Hleq1; subst. *)
+(*       * constructor. *)
+(*       *  *)
+(* Admitted. *)
+
+Lemma tree_leq_tree_leqb {A : Type} `{eq: EqType A} (t1 t2 : tree A) :
+  tree_leq t1 t2 <-> tree_leqb t1 t2 = true.
+Proof. destruct (tree_leqb_spec t1 t2); split; congruence. Qed.
+
+Lemma tree_leq_refl {A : Type} (t : tree A) :
+  tree_leq t t.
+Proof. induction t; constructor; auto; reflexivity. Qed.
+
+Lemma tree_leq_trans {A : Type} (t1 t2 t3 : tree A) :
+  tree_leq t1 t2 -> tree_leq t2 t3 -> tree_leq t1 t3.
+Proof.
+  revert t1 t3; induction t2; intros t1 t3 H0 H1;
+    inversion H0; inversion H1; subst; constructor; auto; lra.
+Qed.
+
+Program Instance OType_tree {A : Type} : OType (tree A) :=
+  {| leq := tree_leq |}.
+Next Obligation.
+  split.
+  - intro; apply tree_leq_refl.
+  - intros ?; eapply tree_leq_trans; eauto.
+Qed.
+
+Inductive free_in {A : Type} : nat -> tree A -> Prop :=
+| free_in_fail : forall n, free_in n (Fail _ n)
+| free_in_choice1 : forall n p t1 t2,
+    free_in n t1 ->
+    free_in n (Choice p t1 t2)
+| free_in_choice2 : forall n p t1 t2,
+    free_in n t2 ->
+    free_in n (Choice p t1 t2)
+| free_in_fix : forall n m t,
+    n <> m ->
+    free_in n t ->
+    free_in n (Fix m t).
+
+Inductive not_free_in {A : Type} : nat -> tree A -> Prop :=
+| not_free_in_leaf : forall n x, not_free_in n (Leaf x)
+| not_free_in_fail : forall n m, n <> m -> not_free_in n (Fail _ m)
+| not_free_in_choice : forall n p t1 t2,
+    not_free_in n t1 ->
+    not_free_in n t2 ->
+    not_free_in n (Choice p t1 t2)
+| not_free_in_fix0 : forall n t,
+    not_free_in n (Fix n t)
+| not_free_in_fix1 : forall n m t,
+    n <> m ->
+    not_free_in n t ->
+    not_free_in n (Fix m t).
+
+Inductive label_in {A : Type} : nat -> tree A -> Prop :=
+| label_in_fail : forall l, label_in l (Fail _ l)
+| label_in_choice1 : forall l p t1 t2,
+    label_in l t1 ->
+    label_in l (Choice p t1 t2)
+| label_in_choice2 : forall l p t1 t2,
+    label_in l t2 ->
+    label_in l (Choice p t1 t2)
+| label_in_fix1 : forall l t,
+    label_in l (Fix l t)
+| label_in_fix2 : forall l m t,
+    l <> m ->
+    label_in l t ->
+    label_in l (Fix m t).
+
+Inductive not_in {A : Type} : nat -> tree A -> Prop :=
+| not_in_leaf : forall n x, not_in n (Leaf x)
+| not_in_fail : forall n m, n <> m -> not_in n (Fail _ m)
+| not_in_choice : forall n p t1 t2,
+    not_in n t1 ->
+    not_in n t2 ->
+    not_in n (Choice p t1 t2)
+| not_in_fix : forall n m t,
+    n <> m ->
+    not_in n t ->
+    not_in n (Fix m t).
+
+Inductive bound_in {A : Type} : nat -> tree A -> Prop :=
+| bound_in_choice1 : forall n p t1 t2,
+    bound_in n t1 ->
+    bound_in n (Choice p t1 t2)
+| bound_in_choice2 : forall n p t1 t2,
+    bound_in n t2 ->
+    bound_in n (Choice p t1 t2)
+| bound_in_fix1 : forall n t,
+    bound_in n (Fix n t)
+| bound_in_fix2 : forall n m t,
+    n <> m ->
+    bound_in n t ->
+    bound_in n (Fix m t).
+
+Inductive not_bound_in {A : Type} : nat -> tree A -> Prop :=
+| not_bound_in_leaf : forall n x, not_bound_in n (Leaf x)
+| not_bound_in_fail : forall n m, not_bound_in n (Fail _ m)
+| not_bound_in_choice : forall n p t1 t2,
+    not_bound_in n t1 ->
+    not_bound_in n t2 ->
+    not_bound_in n (Choice p t1 t2)
+| not_bound_in_fix : forall n m t,
+    n <> m ->
+    not_bound_in n t ->
+    not_bound_in n (Fix m t).
+
+Lemma bound_in_dec {A : Type} (l : nat) (t : tree A) :
+  bound_in l t \/ not_bound_in l t.
+Proof.
+  induction t.
+  - right; constructor.
+  - right; constructor.
+  - destruct IHt1, IHt2.
+    + left; constructor; auto.
+    + left; constructor; auto.
+    + left; apply bound_in_choice2; auto.
+    + right; constructor; auto.
+  - destruct IHt.
+    + left; destruct (Nat.eqb_spec l n); subst; constructor; auto.
+    + destruct (Nat.eqb_spec l n); subst.
+      * left; constructor; auto.
+      * right; constructor; auto.
+Qed.
+
+Lemma free_in_dec {A : Type} (n : nat) (t : tree A) :
+  free_in n t \/ not_free_in n t.
+Proof.
+  induction t.
+  - right; constructor.
+  - destruct (Nat.eqb_spec n n0); subst.
+    + left; constructor.
+    + right; constructor; auto.
+  - destruct IHt1; destruct IHt2.
+    + left; constructor; auto.
+    + left; constructor; auto.
+    + left; apply free_in_choice2; auto.
+    + right; constructor; auto.
+  - destruct IHt.
+    + destruct (Nat.eqb_spec n n0); subst.
+      * right; constructor.
+      * left; constructor; auto.
+    + destruct (Nat.eqb_spec n n0); subst.
+      * right; constructor.
+      * right; constructor; auto.
+Qed.
+
+Lemma label_in_bound_or_free {A : Type} (l : nat) (t : tree A) :
+  label_in l t <-> bound_in l t \/ free_in l t.
+Proof.
+  split.
+  - induction t; intro Hin; inversion Hin; subst.
+    + right; constructor.
+    + destruct (IHt1 H1).
+      * left; constructor; auto.
+      * right; constructor; auto.
+    + destruct (IHt2 H1).
+      * left; apply bound_in_choice2; auto.
+      * right; apply free_in_choice2; auto.
+    + left; constructor.
+    + destruct (IHt H3).
+      * left; constructor; auto.
+      * right; constructor; auto.
+  - induction t; intros [Hbound|Hfree]; try inversion Hbound;
+      try inversion Hfree; subst; try solve [constructor; auto].
+Qed.
+
+Lemma bound_in_label_in {A : Type} (l : nat) (t : tree A) :
+  bound_in l t -> label_in l t.
+Proof. intro; apply label_in_bound_or_free; auto. Qed.
+
+Lemma free_in_label_in {A : Type} (l : nat) (t : tree A) :
+  free_in l t -> label_in l t.
+Proof. intro; apply label_in_bound_or_free; auto. Qed.
+
+Lemma free_in_not_free_in {A : Type} (n : nat) (t : tree A) :
+  ~ free_in n t <-> not_free_in n t.
+Proof.
+  split.
+  - induction t; intro H.
+    + constructor.
+    + destruct (Nat.eqb_spec n n0); subst.
+      * exfalso; apply H; constructor.
+      * constructor; auto.
+    + constructor.
+      * apply IHt1; intro HC; apply H; constructor; auto.
+      * apply IHt2; intro HC; apply H; apply free_in_choice2; auto.
+    + destruct (Nat.eqb_spec n n0); subst; constructor; auto;
+        apply IHt; intro HC; apply H; constructor; auto.
+  - intro H; induction H; intro HC; inversion HC; subst; congruence.
+Qed.
+
+Lemma free_in_not_free_in' {A : Type} (n : nat) (t : tree A) :
+  free_in n t <-> ~ not_free_in n t.
+Proof.
+  split; intro H.
+  - induction H; intro HC; inversion HC; subst; congruence.
+  - revert H. revert n. induction t; intros m H.
+    + exfalso. apply H. constructor.
+    + destruct (Nat.eqb_spec m n); subst.
+      * constructor.
+      * exfalso; apply H; constructor; auto.
+    + destruct (free_in_dec m t1).
+      * constructor; auto.
+      * apply free_in_choice2. apply IHt2.
+        intro HC. apply H. constructor; auto.
+    + destruct (Nat.eqb_spec m n); subst.
+      * exfalso. apply H. constructor.
+      * constructor; auto. apply IHt.
+        intro HC. apply H. constructor; auto.
+Qed.
+
+Lemma bound_in_not_bound_in {A : Type} (n : nat) (t : tree A) :
+  ~ bound_in n t <-> not_bound_in n t.
+Proof.
+  split.
+  - induction t; intro H; try solve [constructor].
+    + constructor.
+      * apply IHt1. intro HC. apply H. constructor; auto.
+      * apply IHt2. intro HC. apply H. apply bound_in_choice2; auto.
+    + destruct (Nat.eqb_spec n n0); subst.
+      * exfalso. apply H. constructor.
+      * constructor; auto. apply IHt.
+        intro HC. apply H. constructor; auto.
+  - intro H. induction H.
+    + intro HC; inversion HC.
+    + intro HC; inversion HC.
+    + intro HC.
+      inversion HC; subst; intuition.
+    + intro HC. inversion HC; subst; congruence.
+Qed.
+
+Lemma not_in_not_bound_in {A : Type} (n : nat) (t : tree A) :
+  not_in n t -> not_bound_in n t.
+Proof.
+  induction t; intro Hnotin; try solve [constructor];
+    inversion Hnotin; subst; constructor; auto.
+Qed.
+
+Lemma not_in_not_free_in {A : Type} (n : nat) (t : tree A) :
+  not_in n t -> not_free_in n t.
+Proof.
+  induction t; intro Hnotin; try solve [constructor];
+    inversion Hnotin; subst; constructor; auto.
+Qed.
+
+Lemma not_in_not_bound_or_free {A : Type} (n : nat) (t : tree A) :
+  not_in n t <-> ~ (free_in n t \/ bound_in n t).
+Proof.
+  split; intro H.
+  - intro HC; induction H; destruct HC as [HC | HC];
+      inversion HC; subst; intuition.
+  - induction t.
+    + constructor.
+    + destruct (Nat.eqb_spec n n0); subst.
+      * exfalso; apply H; left; constructor.
+      * constructor; auto.
+    + constructor.
+      * apply IHt1. intros [HC | HC]; apply H.
+        ** left; constructor; auto.
+        ** right; constructor; auto.
+      * apply IHt2. intros [HC | HC]; apply H.
+        ** left; apply free_in_choice2; auto.
+        ** right; apply bound_in_choice2; auto.
+    + destruct (Nat.eqb_spec n n0); subst.
+      * exfalso. apply H. right; constructor.
+      * constructor; auto. apply IHt. intros [HC | HC]; apply H.
+        ** left; constructor; auto.
+        ** right; constructor; auto.
+Qed.
+
+Lemma not_in_not_bound_and_not_free {A : Type} (n : nat) (t : tree A) :
+  not_in n t <-> not_free_in n t /\ not_bound_in n t.
+Proof.
+  split.
+  - intro Hnotin; apply not_in_not_bound_or_free in Hnotin; split.
+    + apply free_in_not_free_in; intro HC; apply Hnotin; auto.
+    + apply bound_in_not_bound_in; intro HC; apply Hnotin; auto.
+  - intros [Hnotfree Hnotbound].
+    apply not_in_not_bound_or_free; intros [HC|HC].
+    + apply free_in_not_free_in in Hnotfree; auto.
+    + apply bound_in_not_bound_in in Hnotbound; auto.
+Qed.
+
+Lemma label_in_dec {A : Type} (l : nat) (t : tree A) :
+  label_in l t \/ not_in l t.
+Proof.
+  destruct (bound_in_dec l t); destruct (free_in_dec l t);
+    try solve [left; apply label_in_bound_or_free; auto];
+    right; auto; apply not_in_not_bound_and_not_free; auto.
+Qed.
+
+Lemma label_in_not_in {A : Type} (l : nat) (t : tree A) :
+  ~ label_in l t <-> not_in l t.
+Proof.
+  split.
+  - induction t; simpl; intro Hin.
+    + constructor.
+    + constructor; intro HC; subst; apply Hin; constructor.
+    + constructor; try apply IHt1; try apply IHt2;
+        intro HC; apply Hin; solve [constructor; auto].
+    + destruct (Nat.eqb_spec l n); subst.
+      * exfalso; apply Hin; constructor.
+      * constructor; auto; apply IHt;
+          intro HC; apply Hin; constructor; auto.
+  - induction t; intros Hnotin HC;
+      inversion HC; inversion Hnotin; subst; auto.
+    + apply IHt1; auto.
+    + apply IHt2; auto.
+    + apply IHt; auto.
+Qed.
+
+Lemma not_in_label_in {A : Type} (l : nat) (t : tree A) :
+  label_in l t <-> ~ not_in l t.
+Proof.
+  split.
+  - intros Hin Hnotin; apply label_in_not_in in Hnotin; congruence.
+  - intro; apply Decidable.not_not.
+    + destruct (label_in_dec l t); left; auto; congruence.
+    + intro HC. apply label_in_not_in in HC; congruence.
+Qed.
+
+Inductive wf_tree {A : Type} : tree A -> Prop :=
+| wf_leaf : forall x, wf_tree (Leaf x)
+| wf_fail : forall n, wf_tree (Fail _ n)
+| wf_choice : forall p t1 t2,
+    0 <= p <= 1 ->
+    wf_tree t1 -> wf_tree t2 ->
+    wf_tree (Choice p t1 t2)
+| wf_fix : forall n t,
+    wf_tree t ->
+    (* n is not bound by another fix inside t. *)
+    not_bound_in n t ->
+    (* TODO: maybe also any label that is free in t is not also bound
+       in t. *)
+    wf_tree (Fix n t).
+
+(** A strengthened wf predicate.  *)
+Inductive wf_tree' {A : Type} : tree A -> Prop :=
+| wf_leaf' : forall x, wf_tree' (Leaf x)
+| wf_fail' : forall n, wf_tree' (Fail _ n)
+| wf_choice' : forall p t1 t2,
+    0 <= p <= 1 ->
+    wf_tree' t1 -> wf_tree' t2 ->
+    wf_tree' (Choice p t1 t2)
+| wf_fix' : forall n t,
+    wf_tree' t ->
+    (* n is not bound by another fix inside t. *)
+    (forall m, bound_in m t -> (n < m)%nat) ->
+    (forall m, free_in m t -> (m <= n)%nat) ->
+    (* TODO: maybe also any label that is free in t is not also bound
+       in t. *)
+    wf_tree' (Fix n t).
+
+Lemma wf_tree'_wf_tree {A : Type} (t : tree A) :
+  wf_tree' t -> wf_tree t.
+Proof.
+  induction t; simpl; intro Hwf; constructor; inversion Hwf; subst; auto.
+  apply bound_in_not_bound_in; intro HC.
+  apply H2 in HC; lia.
+Qed.
+
+Lemma bound_in_bind {A B : Type} (t : tree A) (k : A -> tree B) (m : nat) :
+  bound_in m (bind t k) ->
+  bound_in m t \/ exists x, bound_in m (k x).
+Proof.
+  simpl; unfold tree_bind; revert m k.
+  induction t; intros m k Hbound; simpl in Hbound.
+  - right. exists a. apply Hbound.
+  - inversion Hbound; subst.
+  - inversion Hbound; subst.
+    + apply IHt1 in H1. destruct H1; intuition.
+      left; constructor; auto.
+    + apply IHt2 in H1. destruct H1; intuition.
+      left. apply bound_in_choice2; auto.
+  - inversion Hbound; subst.
+    left; constructor; auto.
+    apply IHt in H3. destruct H3; intuition.
+    left. constructor; auto.
+Qed.
+
+Lemma bound_in_bind' {A B : Type} (l : nat) (t : tree A) (k : A -> tree B) :
+  bound_in l (bind t k) ->
+  (forall x, not_bound_in l (k x)) ->
+  bound_in l t.
+Proof.
+  intros Hbound Hnotin.
+  apply bound_in_bind in Hbound. destruct Hbound; auto.
+  destruct H. specialize (Hnotin x). apply bound_in_not_bound_in in Hnotin. congruence.
+Qed.
+
+Lemma free_in_bind {A B : Type} (t : tree A) (k : A -> tree B) (m : nat) :
+  free_in m (bind t k) ->
+  free_in m t \/ exists x, free_in m (k x).
+Proof.
+  simpl; unfold tree_bind; revert m k.
+  induction t; intros m k Hfree; simpl in Hfree.
+  - right. exists a. apply Hfree.
+  - inversion Hfree; subst. left; constructor.
+  - inversion Hfree; subst.
+    + apply IHt1 in H1. destruct H1; intuition.
+      left; constructor; auto.
+    + apply IHt2 in H1. destruct H1; intuition.
+      left. apply free_in_choice2; auto.
+  - inversion Hfree; subst. apply IHt in H3. destruct H3; intuition.
+    left. constructor; auto.
+Qed.
+
+Lemma free_in_bind' {A B : Type} (l : nat) (t : tree A) (k : A -> tree B) :
+  free_in l (bind t k) ->
+  (forall x, not_free_in l (k x)) ->
+  free_in l t.
+Proof.
+  intros Hfree Hnotin.
+  apply free_in_bind in Hfree. destruct Hfree; auto.
+  destruct H. specialize (Hnotin x).
+  apply free_in_not_free_in in Hnotin. congruence.
+Qed.
+
+Lemma wf_tree_bind {A B : Type} (t : tree A) (k : A -> tree B) :
+  (forall n x, bound_in n t -> not_bound_in n (k x)) ->
+  wf_tree t ->
+  (forall x, wf_tree (k x)) ->
+  wf_tree (tree_bind t k).
+Proof.
+  unfold tree_bind. revert k.
+  induction t; intros k Hnotbound Hwf_t Hwf_k; simpl; auto.
+  - constructor.
+  - inversion Hwf_t; subst.
+    constructor; auto.
+    + apply IHt1; auto; intros n x Hbound.
+      apply Hnotbound; constructor; auto.
+    + apply IHt2; auto; intros n x Hbound.
+      apply Hnotbound; apply bound_in_choice2; auto.
+  - inversion Hwf_t; subst.
+    eapply IHt in Hwf_k; auto.
+    + constructor; auto.
+      apply bound_in_not_bound_in.
+      intro HC. apply bound_in_bind in HC. destruct HC.
+      * apply bound_in_not_bound_in in H2; congruence.
+      * assert (H0: bound_in n (Fix n t)).
+        { constructor; auto. }
+        destruct H as [x H]. specialize (Hnotbound n x H0).
+        apply bound_in_not_bound_in in Hnotbound. apply Hnotbound; auto.
+    + intros n0 x Hbound. apply Hnotbound.
+      destruct (Nat.eqb_spec n0 n); subst; constructor; auto.
+Qed.
+
+Lemma wf_tree'_bind {A B : Type} (t : tree A) (k : A -> tree B) :
+  (forall n m x, bound_in n t -> bound_in m (k x) -> (n < m)%nat) ->
+  (forall n m x, bound_in n t -> free_in m (k x) -> (m <= n)%nat) ->
+  wf_tree' t ->
+  (forall x, wf_tree' (k x)) ->
+  wf_tree' (tree_bind t k).
+Proof.
+  unfold tree_bind. revert k.
+  induction t; intros k Hbound_lt Hfree_le Hwf_t Hwf_k; simpl; auto.
+  - constructor.
+  - inversion Hwf_t; subst.
+    constructor; auto.
+    + apply IHt1; auto; intros n x Hbound.
+      * intros; eapply Hbound_lt; eauto; constructor; auto.
+      * intros; eapply Hfree_le; eauto; constructor; auto.
+    + apply IHt2; auto; intros n x Hbound.
+      * intros; eapply Hbound_lt; eauto; solve [constructor; auto].
+      * intros; eapply Hfree_le; eauto; solve [constructor; auto].
+  - inversion Hwf_t; subst.
+    eapply IHt in Hwf_k; auto.
+    + constructor; auto.
+      * intros m Hbound.
+        apply bound_in_bind in Hbound. destruct Hbound as [Hbound|Hbound].
+        ++ apply H2; auto.
+        ++ destruct Hbound as [x Hbound].
+           eapply Hbound_lt; eauto; constructor.
+      * intros m Hfree.
+        apply free_in_bind in Hfree. destruct Hfree as [Hfree|Hfree].
+        apply H3; auto.
+        destruct Hfree as [x Hfree].
+        eapply Hfree_le; eauto; constructor.
+    + intros n0 m x Hboundt Hboundk.
+      eapply Hbound_lt; eauto.
+      destruct (Nat.eqb_spec n0 n); subst; constructor; auto.
+    + intros n0 m x Hbound Hfree.
+      eapply Hfree_le; eauto.
+      destruct (Nat.eqb_spec n0 n); subst; constructor; auto.
+Qed.
+
+Lemma not_bound_in_fbind {A : Type} (t1 t2 : tree A) (l m : nat) :
+  not_bound_in m t1 ->
+  not_bound_in m t2 ->
+  not_bound_in m (fbind l t1 t2).
+Proof.
+  revert t2 l m; induction t1; intros t2 l m H0 H1; simpl; auto.
+  - destruct (l =? n); auto.
+  - inversion H0; subst; constructor.
+    + apply IHt1_1; auto.
+    + apply IHt1_2; auto.
+  - inversion H0; subst; constructor; auto.
+    destruct (Nat.eqb_spec n l); subst; auto.
+Qed.
+
+Lemma wf_fbind {A : Type} (t1 t2 : tree A) (l : nat) :
+  wf_tree t1 ->
+  wf_tree t2 ->
+  (forall n, bound_in n t1 -> not_bound_in n t2) ->
+  wf_tree (fbind l t1 t2).
+Proof.
+  revert t2 l. induction t1; intros t2 l Hwf1 Hwf2 Hnotbound; simpl; auto.
+  - destruct (l =? n); auto.
+  - inversion Hwf1; subst. constructor; auto.
+    + apply IHt1_1; auto; intros; apply Hnotbound; constructor; auto.
+    + apply IHt1_2; auto; intros; apply Hnotbound; apply bound_in_choice2; auto.
+  - inversion Hwf1; subst.
+    destruct (Nat.eqb_spec n l); subst; auto.
+    constructor.
+    + apply IHt1; auto; intros; apply Hnotbound.
+      destruct (Nat.eqb_spec n1 n); subst; constructor; auto.
+    + apply not_bound_in_fbind; auto; apply Hnotbound; constructor.
+Qed.
+
+Lemma bound_in_subst_l {A : Type} (t : tree A) (l n m : nat) :
+  bound_in l t <-> bound_in l (subst_l n m t).
+Proof.
+  split; intro Hbound; induction t; inversion Hbound; subst;
+    try solve [apply bound_in_choice2; auto];
+    constructor; auto; destruct (Nat.eqb_spec n0 n); subst; auto.
+Qed.
+
+Lemma not_bound_in_subst_l {A : Type} (t : tree A) (l n m : nat) :
+  not_bound_in l t ->
+  not_bound_in l (subst_l n m t).
+Proof.
+  intros Hnotbound.
+  apply bound_in_not_bound_in.
+  apply bound_in_not_bound_in in Hnotbound.
+  intro HC; apply bound_in_subst_l in HC; auto.
+Qed.
+
+Lemma wf_subst_l {A : Type} (t : tree A) (n m : nat) :
+  wf_tree t ->
+  wf_tree (subst_l n m t).
+Proof.
+  induction t; intro Hwf; simpl; auto.
+  - constructor.
+  - inversion Hwf; subst.
+    constructor; auto.
+  - inversion Hwf; subst.
+    constructor.
+    + destruct (Nat.eqb_spec n0 n); subst; auto.
+    + destruct (Nat.eqb_spec n0 n); subst; auto.
+      apply not_bound_in_subst_l; auto.
+Qed.
+
+Lemma not_bound_in_alpha_convert {A : Type} (t : tree A) (g : nat -> nat) (m : nat) :
+  (forall x y, g x = g y -> x = y) ->
+  not_bound_in m t ->
+  not_bound_in (g m) (alpha_convert g t).
+Proof.
+  revert m.
+  induction t; intros m Hinj Hnotbound; simpl; try solve [constructor].
+  - inversion Hnotbound; subst; constructor; auto.
+  - inversion Hnotbound; subst.
+    constructor. intro HC. apply H2. apply Hinj; auto.
+    apply not_bound_in_subst_l, IHt; auto.
+Qed.
+
+Lemma wf_tree_alpha_convert {A : Type} (t : tree A) (n m : nat) :
+  wf_tree t ->
+  wf_tree (alpha_convert (fun x : nat => (x + n + m)%nat) t).
+Proof.
+  induction t; intro Hwf; simpl; auto.
+  - inversion Hwf; subst; constructor; auto.
+  - inversion Hwf; subst.
+    constructor.
+    + apply wf_subst_l. apply IHt; auto.
+    + apply not_bound_in_subst_l.
+      set (g := fun x => (x + n + m)%nat).
+      assert ((n0 + n + m)%nat = g n0); auto.
+      rewrite H.
+      apply not_bound_in_alpha_convert; auto.
+      unfold g; intuition.
+Qed.
+
+Lemma bound_in_alpha_convert_lt {A : Type} (t : tree A) (l m : nat) :
+  bound_in l (alpha_convert (fun x : nat => (x + m + 1)%nat) t) ->
+  (m < l)%nat.
+Proof.
+  revert l m; induction t; intros l m Hbound;
+    simpl in Hbound; try solve [inversion Hbound].
+  - inversion Hbound; subst.
+    + apply IHt1; auto.
+    + apply IHt2; auto.
+  - inversion Hbound; subst; try lia.
+    apply IHt. apply bound_in_subst_l in H3; auto.
+Qed.
+
+Lemma all_labels_spec {A : Type} (t : tree A) (l : nat) :
+  label_in l t <-> In l (all_labels t).
+Proof.
+  split.
+  - induction t; intro Hbound; inversion Hbound; subst; simpl; auto.
+    + apply nodup_In; apply in_or_app; auto.
+    + apply nodup_In; apply in_or_app; auto.
+    + destruct (in_dec Nat.eq_dec n (all_labels t)).
+      * apply nodup_In; auto.
+      * constructor; auto.
+    + destruct (in_dec Nat.eq_dec n (all_labels t)).
+      * apply nodup_In; auto.
+      * right. apply nodup_In; auto.
+  - induction t; intro Hin.
+    + inversion Hin.
+    + inversion Hin; subst. constructor. inversion H.
+    + simpl in Hin; apply nodup_In, in_app_or in Hin;
+        destruct Hin; try solve [constructor; auto].
+    + destruct (Nat.eqb_spec l n); subst.
+      * constructor.
+      * constructor; auto. apply IHt.
+        simpl in Hin.
+        destruct (in_dec Nat.eq_dec n (all_labels t)).
+        ++ eapply nodup_In; eauto.
+        ++ destruct Hin; subst. congruence.
+           eapply nodup_In; eauto.
+Qed.
+
+Lemma bound_labels_spec {A : Type} (t : tree A) (l : nat) :
+  bound_in l t <-> In l (bound_labels t).
+Proof.
+  split.
+  - induction t; intro Hbound; inversion Hbound; subst; simpl.
+    + apply nodup_In; apply in_or_app; auto.
+    + apply nodup_In; apply in_or_app; auto.
+    + destruct (in_dec Nat.eq_dec n (bound_labels t)).
+      * apply nodup_In; auto.
+      * constructor; auto.
+    + destruct (in_dec Nat.eq_dec n (bound_labels t)).
+      * apply nodup_In; auto.
+      * right. apply nodup_In; auto.
+  - induction t; intro Hin.
+    + inversion Hin.
+    + inversion Hin.
+    + simpl in Hin; apply nodup_In, in_app_or in Hin;
+        destruct Hin; try solve [constructor; auto].
+    + destruct (Nat.eqb_spec l n); subst.
+      * constructor.
+      * constructor; auto. apply IHt.
+        simpl in Hin.
+        destruct (in_dec Nat.eq_dec n (bound_labels t)).
+        ++ eapply nodup_In; eauto.
+        ++ destruct Hin; subst. congruence.
+           eapply nodup_In; eauto.
+Qed.
+
+Lemma bound_labels_leq_all_labels {A : Type} :
+  leq (@bound_labels A) all_labels.
+Proof.
+  intros t n H; apply bound_labels_spec in H;
+    apply all_labels_spec; apply bound_in_label_in; auto.
+Qed.
+
+Lemma wf_tree_fbind_alpha_convert {A : Type} (t1 t2 : tree A) (l : nat) :
+  wf_tree t1 ->
+  wf_tree t2 ->
+  (forall m, bound_in m t2 -> bound_in m t1) ->
+  wf_tree
+    (fbind l t1
+           (alpha_convert
+              (fun x : nat => (x + list_max (all_labels t1) + 1)%nat) t2)).
+Proof.
+  intros. apply wf_fbind; auto.
+  - apply wf_tree_alpha_convert; auto.
+  - intros n Hbound; apply bound_in_not_bound_in.
+    intro HC; apply bound_in_alpha_convert_lt in HC.
+    apply bound_in_label_in in Hbound.
+    apply all_labels_spec in Hbound.
+    apply list_max_spec in Hbound. lia.
+Qed.
+
+Lemma bound_in_fbind {A : Type} (t1 t2 : tree A) (l m : nat) :
+  bound_in m t1 ->
+  bound_in m (fbind l t1 t2).
+Proof.
+  induction t1; intros Hbound; inversion Hbound; subst;
+    try solve [apply bound_in_choice2; auto];
+    constructor; auto; destruct (Nat.eqb_spec n l); subst; auto.
+Qed.
+
+Lemma tree_chain_wf {A : Type} (t : tree A) (l i : nat) :
+  wf_tree t ->
+  wf_tree (tree_chain t l i).
+Proof.
+  revert l t.
+  induction i; intros l t Hwf; auto.
+  simpl.
+  apply wf_tree_fbind_alpha_convert; auto.
+  intros m Hbound. clear IHi.
+  induction i; auto; simpl.
+  apply bound_in_fbind; auto.
+Qed.
+
+Lemma fbind_assoc {A : Type} (t1 t2 t3 : tree A) (n : nat) :
+  fbind n t1 (fbind n t2 t3) = fbind n (fbind n t1 t2) t3.
+Proof.
+  revert t2 t3 n. induction t1; intros t2 t3 m; simpl.
+  - reflexivity.
+  - destruct (Nat.eqb_spec m n); subst; simpl.
+    + reflexivity.
+    + destruct (Nat.eqb_spec m n); subst; congruence; reflexivity.
+  - rewrite IHt1_1, IHt1_2; reflexivity.
+  - destruct (Nat.eqb_spec n m); subst.
+    + reflexivity.
+    + rewrite IHt1; reflexivity.
+Qed.
+
+Lemma not_in_subst_l {A : Type} (t : tree A) (l m n : nat) :
+  n <> m ->
+  not_in m t ->
+  not_in m (subst_l l n t).
+Proof.
+  induction t; intros Hneq Hnotin; simpl; auto; inversion Hnotin; subst.
+  - destruct (Nat.eqb_spec n0 l); subst; constructor; auto.
+  - constructor; auto.
+  - constructor; auto.
+    destruct (Nat.eqb_spec n0 l); subst; auto.
+Qed.
+
+Lemma not_free_in_subst_l {A : Type} (t : tree A) (l m : nat) :
+  l <> m ->
+  not_free_in l (subst_l l m t).
+Proof.
+  induction t; intro Hneq; simpl.
+  - constructor.
+  - constructor; destruct (Nat.eqb_spec n l); subst; auto.
+  - constructor; auto.
+  - destruct (Nat.eqb_spec n l); subst; constructor; auto.
+Qed.
+
+(** Subtlety here: what happens when (g m) is bound somewhere? Then it
+   may appear free under that binder without violating (not_free_in (g
+   m) t). However, when we alpha convert that bound occurrence of (g
+   m) we also replace all free occurrences underneath it so that it
+   doesn't become free in the overall tree. *)
+Lemma not_in_alpha_convert {A : Type} (t : tree A) (g : nat -> nat) (m : nat) :
+  (forall x, x <> g x) ->
+  (forall x y, g x = g y -> x = y) ->
+  not_bound_in m t ->
+  not_free_in (g m) t ->
+  not_in (g m) (alpha_convert g t).
+Proof.
+  induction t; intros Hneq Hinj Hnotbound Hnotin; simpl.
+  - constructor.
+  - inversion Hnotin; subst. constructor; auto.
+  - inversion Hnotbound; inversion Hnotin; subst. constructor.
+    + apply IHt1; auto.
+    + apply IHt2; auto.
+  - 
+    destruct (Nat.eqb_spec (g m) n); subst.
+    + constructor; auto.
+      apply not_in_not_bound_and_not_free. split.
+      * apply not_free_in_subst_l; auto.
+      * inversion Hnotbound; subst.
+        apply not_bound_in_subst_l.
+        apply not_bound_in_alpha_convert; auto.
+    + inversion Hnotbound; subst. constructor; auto.
+      apply not_in_subst_l ; auto.
+      apply IHt; auto.
+      inversion Hnotin; subst; auto; congruence.
+Qed.
+
+Lemma not_in_alpha_convert' {A : Type} (t : tree A) (g : nat -> nat) (m : nat) :
+  (forall x y, g x = g y -> x = y) ->
+  not_bound_in m t ->
+  not_in (g m) t ->
+  not_in (g m) (alpha_convert g t).
+Proof.
+  induction t; intros Hinj Hnotbound Hnotin; simpl.
+  - constructor.
+  - inversion Hnotin; subst. constructor; auto.
+  - inversion Hnotbound; inversion Hnotin; subst. constructor.
+    + apply IHt1; auto.
+    + apply IHt2; auto.
+  - inversion Hnotbound; subst.
+    constructor. intuition.
+    apply not_in_subst_l; auto.
+    apply IHt; auto.
+    inversion Hnotin; subst; auto.    
+Qed.
+
+Lemma bound_in_lt_not_bound_in {A : Type} (t : tree A) (m : nat) :
+  (forall x, bound_in x t -> (m < x)%nat) ->
+  not_bound_in m t.
+Proof.
+  induction t; intro Hlt; simpl.
+  - constructor.
+  - constructor.
+  - constructor.
+    + apply IHt1; intros x Hbound; apply Hlt; constructor; auto.
+    + apply IHt2; intros x Hbound; apply Hlt; apply bound_in_choice2; auto.
+  - destruct (Nat.eqb_spec m n); subst.
+    + specialize (Hlt n (bound_in_fix1 _ _)); lia.
+    + constructor; auto. apply IHt. intros x Hbound; apply Hlt.
+      destruct (Nat.eqb_spec x n); subst; constructor; auto.
+Qed.
+
+Lemma bound_in_alpha_convert_exists {A : Type} (t : tree A) (f : nat -> nat) (l : nat) :
+  bound_in l (alpha_convert f t) ->
+  exists m, bound_in m t /\ f m = l.
+Proof.
+  induction t; intro Hbound; inversion Hbound; subst.
+  - apply IHt1 in H1; destruct H1 as [m [H1 H2]]; subst.
+    exists m; split; auto; constructor; auto.
+  - apply IHt2 in H1; destruct H1 as [m [H1 H2]]; subst.
+    exists m; split; auto; apply bound_in_choice2; auto.
+  - exists n; split; auto; constructor.
+  - apply bound_in_subst_l in H3. apply IHt in H3.
+    destruct H3 as [m [H3 H4]]; subst.
+    exists m. split; auto.
+    destruct (Nat.eqb_spec m n); subst; constructor; auto.
+Qed.  
+Lemma bound_in_tree_chain {A : Type} (t : tree A) (l m n : nat) :
+  bound_in l t ->
+  bound_in l (tree_chain t m n).
+Proof.
+  induction n; simpl; auto; intros; apply bound_in_fbind; auto.
+Qed.
+
+Lemma list_max_lt_not_in {A : Type} (t : tree A) (m : nat) :
+  (list_max (all_labels t) < m)%nat ->
+  not_in m t.
+Proof.
+  intro Hlt.
+  apply label_in_not_in; intro HC.
+  apply all_labels_spec in HC.
+  apply list_max_spec in HC. lia.
+Qed.
+
+Lemma list_max_subset (l1 l2 : list nat) :
+  (forall x, In x l1 -> In x l2) -> (* l1 ⊆ l2 *)
+  (list_max l1 <= list_max l2)%nat.
+Proof.
+  induction l1; intro Hsubset; simpl.
+  - lia.
+  - destruct (Nat.leb_spec0 a (list_max l1)).
+    + rewrite Nat.max_r; auto. apply IHl1.
+      intros x Hin. apply Hsubset. right; auto.
+    + rewrite Nat.max_l; try lia.
+      apply list_max_spec; apply Hsubset; constructor; reflexivity.
+Qed.
+
+Lemma tree_leq_fbind {A : Type} (t1 t2 : tree A) (l : nat) :
+  tree_leq t1 (fbind l t1 t2).
+Proof.
+  induction t1; simpl.
+  - constructor.
+  - destruct (Nat.eqb_spec l n); subst; constructor.
+  - constructor; auto; reflexivity.
+  - constructor.
+    destruct (Nat.eqb_spec n l); subst; auto; apply tree_leq_refl.
+Qed.
+
+Lemma tree_leq_tree_chain {A : Type} (t : tree A) (l n : nat) :
+  tree_leq t (tree_chain t l n).
+Proof.
+  induction n; simpl.
+  - apply tree_leq_refl.
+  - eapply tree_leq_trans; eauto. apply tree_leq_fbind.
+Qed.
+
+Lemma in_bound_labels_choice1 {A : Type} (t1 t2 : tree A) (p : Q) (x : nat) :
+  In x (bound_labels t1) ->
+  In x (bound_labels (Choice p t1 t2)).
+Proof.
+  intro Hin; apply bound_labels_spec in Hin.
+  apply bound_labels_spec; constructor; auto.
+Qed.
+
+Lemma in_bound_labels_choice2 {A : Type} (t1 t2 : tree A) (p : Q) (x : nat) :
+  In x (bound_labels t2) ->
+  In x (bound_labels (Choice p t1 t2)).
+Proof.
+  intro Hin; apply bound_labels_spec in Hin.
+  apply bound_labels_spec; solve [constructor; auto].
+Qed.
+
+Lemma in_bound_labels_fix1 {A : Type} (t : tree A) (x : nat) :
+  In x (bound_labels (Fix x t)).
+Proof. apply bound_labels_spec; constructor. Qed.
+
+Lemma in_bound_labels_fix2 {A : Type} (t : tree A) (l x : nat) :
+  In x (bound_labels t) ->
+  In x (bound_labels (Fix l t)).
+Proof.
+  intro Hin; apply bound_labels_spec in Hin.
+  apply bound_labels_spec.
+  destruct (Nat.eqb_spec x l); subst; constructor; auto.
+Qed.
+
+Lemma bound_in_monotone {A : Type} (t1 t2 : tree A) (x : nat) :
+  tree_leq t1 t2 -> bound_in x t1 -> bound_in x t2.
+Proof.
+  intros Hleq; induction Hleq; intro Hbound; auto;
+    inversion Hbound; subst; solve [constructor; auto].
+Qed.
+
+Lemma bound_labels_monotone {A : Type} : monotone (@bound_labels A).
+  intros t1 t2 Hleq x Hin.
+  apply bound_labels_spec.
+  eapply bound_in_monotone; eauto.
+  apply bound_labels_spec; auto.
+Qed.
+
+(** free_labels isn't monotone in general. Considering the following
+    case: t1 = Fail 0, t2 = Leaf x. We have t1 <= t2 with label 0
+    appearing free in t1 but not in t2. However, we can prove this
+    specifically for fbind l t1 t2 if we know that l appears free in
+    t2. *)
+Lemma free_in_fbind {A : Type} (t1 t2 : tree A) (l x : nat) :
+  free_in l t2 -> free_in x t1 -> free_in x (fbind l t1 t2).
+Proof.
+  induction t1; intros H0 H1; simpl; auto;
+    inversion H1; subst; try solve [constructor; auto].
+  - destruct (Nat.eqb_spec l n); subst; auto.
+  - constructor; auto; destruct (Nat.eqb_spec n l); subst; auto.
+Qed.
+
+Lemma free_in_subst_l {A : Type} (t : tree A) (l x y : nat) :
+  l <> x ->
+  free_in l t -> free_in l (subst_l x y t).
+Proof.
+  induction t; intros Hneq Hfree; simpl; auto; inversion Hfree; subst.
+  - destruct (Nat.eqb_spec n x); subst; auto; congruence.
+  - constructor; auto.
+  - solve [constructor; auto].
+  - constructor; auto.
+    destruct (Nat.eqb_spec n x); subst; auto.
+Qed.
+
+Lemma free_in_subst_l' {A : Type} (t : tree A) (l x y : nat) :
+  l <> y ->
+  free_in l (subst_l x y t) -> free_in l t.
+Proof.
+  induction t; intros Hneq Hfree; simpl; auto; inversion Hfree; subst.
+  - destruct (Nat.eqb_spec n x); subst; try constructor; congruence.
+  - constructor; auto.
+  - solve [constructor; auto].
+  - constructor; auto.
+    destruct (Nat.eqb_spec n x); subst; auto.
+Qed.
+
+(** In general, x can get captured and become not free if there is
+    some bound variable l such that g l = x. The two preconditions
+    here are sufficient to know that won't happen. *)
+Lemma free_in_alpha_convert {A : Type} (g : nat -> nat) (t : tree A) (x : nat) :
+  wf_tree' t ->
+  (forall y, (y < g y)%nat) ->
+  free_in x t <-> free_in x (alpha_convert g t).
+Proof.
+  intros Hwf Hlt; split.
+  - induction t; intro Hfree; simpl; auto; inversion Hwf; subst.
+    + inversion Hfree; subst; solve [constructor; auto].
+    + inversion Hfree; subst.
+      apply IHt in H1; auto.
+      apply H3 in H6.
+      destruct (Nat.eqb_spec x (g n)); subst.
+      * specialize (Hlt n); lia.
+      * constructor; auto.
+        apply free_in_subst_l; auto.
+  - induction t; intro Hfree; simpl in *; auto;
+      inversion Hfree; subst; inversion Hwf; subst.
+    + constructor; auto.
+    + solve [constructor; auto].
+    + destruct (Nat.eqb_spec x n); subst.
+      * apply free_in_not_free_in' in H3; exfalso; apply H3.
+        apply not_free_in_subst_l; auto.
+      * constructor; auto.
+        apply IHt; auto.
+        apply free_in_subst_l' in H3; auto.
+Qed.
+
+Lemma not_free_fbind {A : Type} (t1 t2 : tree A) (l : nat) :
+  not_free_in l t1 ->
+  fbind l t1 t2 = t1.
+Proof.
+  induction t1; intro Hnotfree; simpl; auto.
+  - destruct (Nat.eqb_spec l n); subst; auto.
+    inversion Hnotfree; congruence.
+  - inversion Hnotfree; subst.
+    rewrite IHt1_1; auto; rewrite IHt1_2; auto.
+  - inversion Hnotfree; subst.
+    + rewrite Nat.eqb_refl; reflexivity.
+    + destruct (Nat.eqb_spec n l); subst.
+      * congruence.
+      * rewrite IHt1; auto.
+Qed.
+
+Lemma not_free_tree_chain {A : Type} (t : tree A) (l n : nat) :
+  not_free_in l t ->
+  not_free_in l (tree_chain t l n).
+Proof.
+  induction n; simpl; auto; intro Hnotfree.
+  rewrite not_free_fbind; auto.
+Qed.
+
+Lemma tree_chain_const {A : Type} (t : tree A) (l n : nat) :
+  not_free_in l t -> tree_chain t l n = t.
+Proof.
+  induction n; simpl; auto.
+  intro Hnotfree.
+  rewrite not_free_fbind; auto.
+  rewrite IHn; auto.
+Qed.
+
+(** If x is free in t, then x is free along the entire chain generated
+    from t. When the generating label l doesn't appear in t, the chain
+    is constant so the result is trivial. Otherwise it follows from
+    relatively straightforward induction on t. *)
+Lemma free_in_tree_chain {A : Type} (t : tree A) (l n x : nat) :
+  wf_tree' t ->
+  free_in x t -> free_in x (tree_chain t l n).
+Proof.
+  intro Hwf.
+  destruct (free_in_dec l t) eqn:H0.
+  - induction n; simpl; auto; intro H1.
+    apply free_in_fbind; auto.
+    apply free_in_alpha_convert; auto.
+    intro y; lia.
+  - intro Hfree.
+    rewrite tree_chain_const; auto.
+Qed.
+
+Lemma all_labels_tree_chain_subset {A : Type} (t : tree A) (l n x : nat) :
+  wf_tree' t ->
+  In x (all_labels t) -> In x (all_labels (tree_chain t l n)).
+Proof.
+  intros Hwf Hin.
+  apply all_labels_spec in Hin.
+  apply label_in_bound_or_free in Hin.
+  apply all_labels_spec.
+  apply label_in_bound_or_free.
+  destruct Hin as [Hbound|Hfree].
+  - left; eapply bound_in_monotone; eauto; apply tree_leq_tree_chain.
+  - right; apply free_in_tree_chain; auto.
+Qed.
+
+(** The other direction is true as long as renaming via g doesn't
+    capture any free variables (forall m, bound_in m t -> not_free_in
+    (g m) t). *)
+Lemma not_free_in_alpha_convert {A : Type} (t : tree A) (g : nat -> nat) (l : nat) :
+  not_free_in l t -> not_free_in l (alpha_convert g t).
+Proof.
+  induction t; intro Hnotfree; simpl; auto; inversion Hnotfree; subst.
+  - constructor; auto.
+  - destruct (Nat.eqb_spec n (g n)).
+    + rewrite <- e; constructor.
+    + constructor; auto.
+      apply not_free_in_subst_l; auto.
+  - destruct (Nat.eqb_spec l (g n)); subst.
+    + constructor.
+    + constructor; auto.
+      apply free_in_not_free_in; intro HC.
+      apply free_in_subst_l' in HC; auto.
+      apply IHt in H3; apply free_in_not_free_in in H3.
+      congruence.
+Qed.
+
+Lemma bound_in_fbind_or {A : Type} (t1 t2 : tree A) (l m : nat) :
+  bound_in m (fbind l t1 t2) ->
+  bound_in m t1 \/ bound_in m t2.
+Proof.
+  induction t1; simpl; intro Hbound.
+  - left; auto.
+  - destruct (Nat.eqb_spec l n); subst.
+    + right; auto.
+    + inversion Hbound.
+  - inversion Hbound; subst.
+    + apply IHt1_1 in H1; destruct H1.
+      * left; constructor; auto.
+      * right; auto.
+    + apply IHt1_2 in H1; destruct H1.
+      * left; solve [constructor; auto].
+      * right; auto.
+  - destruct (Nat.eqb_spec n l); subst.
+    + left; auto.
+    + inversion Hbound; subst.
+      * left; constructor.
+      * apply IHt1 in H3; destruct H3.
+        ++ left; constructor; auto.
+        ++ right; auto.
+Qed.
+
+(** If something is bound in the chain generated from t, then
+    something must be bound in t. This is useful in conjunction with
+    the following lemma [bound_in_tree_chain_lt]. *)
+Lemma bound_in_tree_chain_exists {A : Type} (t : tree A) (l i m : nat) :
+  bound_in m (tree_chain t l i) ->
+  exists n, bound_in n t.
+Proof.
+  induction i; simpl; intro Hbound.
+  - exists m; auto.
+  - apply bound_in_fbind_or in Hbound.
+    destruct Hbound as [Hbound|Hbound]; auto.
+    apply bound_in_alpha_convert_exists in Hbound; firstorder.
+Qed.
+
+(** If m is bound in a chain generated from t, then either m is bound
+    in t or it's strictly larger than anything bound in t. *)
+Lemma bound_in_tree_chain_lt {A : Type} (t : tree A) (l m i : nat) :
+  wf_tree' t ->
+  bound_in m (tree_chain t l i) ->
+  bound_in m t \/ (forall y, bound_in y t -> (y < m)%nat).
+Proof.
+  induction i; simpl; intros Hwf Hbound; auto.
+  apply bound_in_fbind_or in Hbound; destruct Hbound as [Hbound|Hbound].
+  apply IHi in Hbound; auto.
+  right. intros y Hboundy.
+  apply bound_in_alpha_convert_lt in Hbound.
+  apply bound_in_label_in in Hboundy.
+  apply all_labels_spec in Hboundy.
+  apply list_max_spec in Hboundy.
+  assert (Hle: (list_max (all_labels t) <=
+                list_max (all_labels (tree_chain t l i)))%nat).
+  { apply list_max_monotone; intro x;
+      apply all_labels_tree_chain_subset; auto. }
+  lia.
+Qed.
+
+Lemma free_in_bound_in_chain_lt {A : Type} (t : tree A) (i : nat) :
+  wf_tree' t ->
+  (forall n m, free_in n t -> bound_in m t -> (n < m)%nat) ->
+  forall n m l, free_in n t -> bound_in m (tree_chain t l i) -> (n < m)%nat.
+Proof.
+  intros Hwf Hlt n m l Hfree Hbound; pose proof Hbound as Hbound'.
+  apply bound_in_tree_chain_exists in Hbound; destruct Hbound as [o Hbound].
+  apply bound_in_tree_chain_lt in Hbound'; destruct Hbound'; auto.
+  specialize (H _ Hbound); transitivity o; auto.
+Qed.
+
+Lemma not_bound_in_alpha_convert_lt {A : Type} (t : tree A) (g : nat -> nat) (m : nat) :
+  (forall x, (m < g x)%nat) ->
+  not_bound_in m (alpha_convert g t).
+Proof.
+  induction t; intro Hlt; simpl; try solve [constructor; auto].
+  - destruct (Nat.eqb_spec m (g n)); subst.
+    + specialize (Hlt n); lia.
+    + constructor; auto; apply not_bound_in_subst_l; auto.
+Qed.
+
+Lemma not_free_in_tree_chain {A : Type} (t : tree A) (l n : nat) :
+  not_free_in l t ->
+  tree_chain t l n = t.
+Proof.
+  induction n; simpl; auto; intro Hnotfree.
+  rewrite IHn; auto.
+  apply not_free_fbind; auto.
+Qed.
+
+(* Lemma in_bound_labels_fbind1 {A : Type} (t1 t2 : tree A) (l x : nat) : *)
+(*   In x (bound_labels t1) -> *)
+(*   In x (bound_labels (fbind l t1 t2)). *)
+(* Proof. *)
+(*   induction t1; intro Hin; simpl. *)
+(*   - inversion Hin. *)
+(*   - inversion Hin. *)
+(*   - apply nodup_In. *)
+(*     apply bound_labels_spec in Hin. *)
+(*     apply in_or_app. *)
+(*     inversion Hin; subst. *)
+(*     + left; apply IHt1_1; apply bound_labels_spec; auto. *)
+(*     + right; apply IHt1_2; apply bound_labels_spec; auto. *)
+(*   - apply bound_labels_spec in Hin. *)
+(*     inversion Hin; subst. *)
+(*     + destruct (Nat.eqb_spec n l); subst. *)
+(*       * destruct (in_dec Nat.eq_dec l (bound_labels t1)). *)
+(*         ++ apply nodup_In; auto. *)
+(*         ++ left; auto. *)
+(*       * destruct (in_dec Nat.eq_dec n (bound_labels (fbind l t1 t2))). *)
+(*         ++ apply nodup_In; auto. *)
+(*         ++ left; auto. *)
+(*     + destruct (Nat.eqb_spec n l); subst. *)
+(*       * destruct (in_dec Nat.eq_dec l (bound_labels t1)). *)
+(*         ++ apply nodup_In; auto; apply bound_labels_spec; auto. *)
+(*         ++ right; apply nodup_In; apply bound_labels_spec; auto. *)
+(*       * destruct (in_dec Nat.eq_dec n (bound_labels (fbind l t1 t2))). *)
+(*         ++ apply nodup_In; apply IHt1; apply bound_labels_spec; auto. *)
+(*         ++ right; apply nodup_In; apply IHt1; apply bound_labels_spec; auto. *)
+(* Qed. *)
+
+Lemma in_not_bound_choice1 {A : Type} (t1 t2 : tree A) (p : Q) (l : list nat) :
+  (forall x : nat, In x l -> not_bound_in x (Choice p t1 t2)) ->
+  forall x : nat, In x l -> not_bound_in x t1.
+Proof.
+  intros H x Hin. specialize (H x Hin); inversion H; subst; auto.
+Qed.
+
+Lemma in_not_bound_choice2 {A : Type} (t1 t2 : tree A) (p : Q) (l : list nat) :
+  (forall x : nat, In x l -> not_bound_in x (Choice p t1 t2)) ->
+  forall x : nat, In x l -> not_bound_in x t2.
+Proof.
+  intros H x Hin. specialize (H x Hin); inversion H; subst; auto.
+Qed.
+
+Lemma bound_in_tree_bind {A B : Type} (t : tree A) (k : A -> tree B) (l : nat) :
+  bound_in l t -> 
+  bound_in l (tree_bind t k).
+Proof.
+  unfold tree_bind; induction t; simpl; intro Hbound;
+    inversion Hbound; subst; try solve [constructor; auto].
+Qed.
+
+Lemma wf_tree_bind' {A B : Type} (t : tree A) (k : A -> tree B) :
+  wf_tree (tree_bind t k) ->
+  wf_tree t.
+Proof.
+  unfold tree_bind; induction t; simpl; intro Hwf;
+    inversion Hwf; subst; try solve [constructor; auto].
+  - constructor; auto.
+    apply bound_in_not_bound_in; intro HC.
+    apply bound_in_not_bound_in in H2; apply H2.
+    apply bound_in_tree_bind; auto.
+Qed.
